feat(lts): WIP --- trace theory
- lammas about traces and their states
- WIP --- sim_traces proof

theories/concur/lts.v
@@ -42,7 +42,7 @@ Section ClassDef.
 Record mixin_of (S0 : Type) (L : Type)
                 (sb : Equality.class_of S0)
                 (S := Equality.Pack sb) := Mixin {
-  tr : L -> rel S;
+  trans : L -> rel S;
 }.
 
 Set Primitive Projections.
@@ -88,16 +88,16 @@ Notation LTSType S L m := (@LTS.pack S L _ _ id m).
 Section Def.
 Context {L : Type} (S : ltsType L).
 
-Definition tr : L -> rel S := LTS.tr (LTS.class S).
+Definition trans : L -> rel S := LTS.trans (LTS.class S).
 
 End Def.
 
 Module Export Syntax.
-Notation "s1 '--[' l ']-->' s2" := (tr l s1 s2) : lts_scope.
-Notation "s1 '-->' s2"  := (exlab tr)   : lts_scope.
-Notation "s1 '-->?' s2" := (exlab tr)^? : lts_scope.
-Notation "s1 '-->+' s2" := (exlab tr)^+ : lts_scope. 
-Notation "s1 '-->*' s2" := (exlab tr)^* : lts_scope.
+Notation "s1 '--[' l ']-->' s2" := (trans l s1 s2) : lts_scope.
+Notation "s1 '-->' s2"  := (exlab trans)   : lts_scope.
+Notation "s1 '-->?' s2" := (exlab trans)^? : lts_scope.
+Notation "s1 '-->+' s2" := (exlab trans)^+ : lts_scope. 
+Notation "s1 '-->*' s2" := (exlab trans)^* : lts_scope.
 End Syntax.
 
 End LTS.
@@ -107,20 +107,28 @@ End LTS.
 (* Check (s1 --[l]--> s2). *)
 
 Module Export Step. 
+
 Section Def.
 Context {L : Type} (S : ltsType L).
 
-Structure step : Type := mk_step { 
+Record step : Type := mk_step {
   lbl : L; src : S; dst : S;  
-  _   : src --[lbl]--> dst;
 }.
 
-Definition linkable : rel step := 
+Definition is_step : pred step := 
+  fun s => (src s) --[lbl s]--> (dst s).
+
+(* TODO: better name? *)
+Definition lnk : rel step := 
   fun s t => dst s == src t. 
+
+Definition rev_step : step -> step := 
+  fun s => mk_step (lbl s) (dst s) (src s).
 
 End Def.
 
 Prenex Implicits lbl src dst.
+Prenex Implicits is_step lnk rev_step.
 
 Section EQ. 
 Context {L : eqType} (S : ltsType L).
@@ -131,45 +139,200 @@ Definition prod_of_step : step S -> L * S * S :=
 Lemma prod_of_step_inj : injective prod_of_step.
 Proof. 
   rewrite /prod_of_step; move=> x y /= []. 
-  case x=> l1 s1 d1 H1; case y=> l2 s2 d2 H2 /=. 
-  move=> Hl Hs Hd; move: H1 H2; rewrite Hl Hs Hd=> H1 H2.
-  have ->: H1 = H2=> //.
-  exact/bool_irrelevance.
+  by case x; case y=> /= ?????? -> -> ->. 
 Qed.
 
 Definition step_eqMixin := InjEqMixin prod_of_step_inj.
 Canonical step_eqType := Eval hnf in EqType (step S) step_eqMixin.
 
+(* Lemma prod_of_step_inj : injective (prod_of_step : step S -> L * S * S). *)
+(* Proof.  *)
+(*   case=> [s1 H1]; case=> [s2 H2] /=. *)
+(*   move=> /prod_of_step_tup_inj. *)
+(*   move: H2=> /[swap]; move: H1=> /[swap] -> H1 H2. *)
+(*   have ->: H1 = H2=> //; exact/bool_irrelevance. *)
+(* Qed. *)
+
+(* Definition step_eqMixin := InjEqMixin prod_of_step_inj. *)
+(* Canonical step_eqType := Eval hnf in EqType (step S) step_eqMixin. *)
+
 End EQ.
+
+Section Theory.
+Context {L : Type} (S : ltsType L).
+Implicit Types (st : step S).
+
+Lemma lnk_rev st : lnk st (rev_step st).
+Proof. by rewrite /lnk. Qed.
+
+Lemma rev_lnk st : lnk (rev_step st) st.
+Proof. by rewrite /lnk. Qed.
+
+End Theory.
+
 End Step.
 
 
-Module Export FinTrace. 
+Module Export Trace. 
+
+Notation trace_seq S := (seq (step S)).
+
 Section Def. 
 Context {L : Type} (S : ltsType L).
 
-Structure ftrace : Type := FinTrace { 
-  ftrace_val :> seq (step S); 
-  _          :  sorted (@linkable L S) ftrace_val;
+Definition is_trace : pred (trace_seq S) := 
+  fun s => (all is_step s) && (sorted lnk s).
+
+Structure trace : Type := Trace { 
+  trace_val :> trace_seq S; 
+  _         :  is_trace trace_val;
 }.
 
-Definition labels : ftrace -> seq L := map lbl. 
+Canonical trace_subType := Eval hnf in [subType for trace_val].
 
-Definition states : ftrace -> seq S := 
-  fun tr => 
-    let hd := omap src (ohead tr) in
-    let tl := map dst tr in
-    ocons hd tl.
+Implicit Types (tr : trace).
 
-Definition ftraces_at : S -> pred ftrace := 
+Lemma trace_steps tr : all is_step tr.
+Proof. by case: tr; rewrite /is_trace=> ? /= /andP[]. Qed.
+
+Lemma trace_lnk tr : sorted lnk tr.
+Proof. by case: tr; rewrite /is_trace=> ? /= /andP[]. Qed.
+
+(* TODO: better name? *)
+Definition joint : rel (trace_seq S) := 
+  fun s1 s2 => 
+    match s2 with 
+    | [::]      => true
+    | st :: s2 => lnk (last (rev_step st) s1) st
+    end.
+
+Definition labels : trace_seq S -> seq L := map lbl. 
+
+Definition states : trace_seq S -> seq S := 
+  fun s => 
+    match s with 
+    | [::]    => [::]
+    | st :: s => src st :: dst st :: map dst s
+    end. 
+
+Definition traces_at : S -> pred trace := 
   fun s tr => s == head s (states tr).
 
 (* TODO: this is actually a fmap on (A -> Prop) functor. *)
-Definition lts_lang : S -> lang L := 
-  fun s w => exists tr, w = labels tr /\ ftraces_at s tr.
+Definition ltslang : S -> lang L := 
+  fun s w => exists tr, w = labels tr /\ traces_at s tr.
+
+Definition mk_trace tr mkTr : trace :=
+  mkTr (let: Trace _ trP := tr return is_trace tr in trP).
 
 End Def. 
-End FinTrace.
+
+Arguments joint : simpl never.
+
+Section Seq.
+Context {L : Type} (S : ltsType L).
+Implicit Types (st : step S) (s : trace_seq S) (tr : trace S).
+
+Lemma nil_traceP : is_trace ([::] : seq (step S)).
+Proof. done. Qed.
+Canonical nil_trace := Trace nil_traceP.
+
+End Seq.
+
+Notation "[ 'trace' 'of' tr ]" := (mk_trace (fun trP => @Trace _ _ tr trP))
+  (at level 0, format "[ 'trace'  'of'  tr ]") : form_scope.
+
+Notation "[ 'trace' ]" := [trace of [::]]
+  (at level 0, format "[ 'trace' ]") : form_scope.
+
+Section EQ.
+Context {L : eqType} (S : ltsType L).
+
+Definition trace_eqMixin := Eval hnf in [eqMixin of trace S by <:].
+Canonical trace_eqType := Eval hnf in EqType (trace S) trace_eqMixin.
+
+End EQ.
+
+Section Theory. 
+Context {L : Type} (S : ltsType L).
+Implicit Types (st : step S) (s : trace_seq S) (tr : trace S).
+
+Lemma joint0s s :
+  joint [::] s.
+Proof. by rewrite /joint; case: s=> [|??] //=; rewrite rev_lnk. Qed.
+
+Lemma joints0 s :
+  joint s [::].
+Proof. by rewrite /joint. Qed.
+
+Lemma joint_cons st s1 s2 :
+  joint s1 (st :: s2) = joint s1 [:: st]. 
+Proof. by rewrite /joint; case: s2=> [|??] //=; rewrite last_rcons. Qed.
+
+Lemma joint_rcons st s1 s2 :
+  joint (rcons s1 st) s2 = joint [:: st] s2. 
+Proof. by rewrite /joint; case: s2=> [|??] //=; rewrite last_rcons. Qed.
+
+Lemma cons_is_trace st s : 
+  is_step st -> joint [:: st] s -> is_trace s -> is_trace (st :: s).
+Proof. 
+  move=> Hs Hj Htr; rewrite /is_trace /=.
+  repeat (apply/andP; split)=> //.
+  - by move: Htr; rewrite /is_trace=> /andP[]. 
+  move: Hj Htr; case: s=> [|st' {}s] //=.
+  rewrite joint_cons /joint /= => Hlnk.
+  rewrite /is_trace /= => /andP[/andP[]].
+  move=> ???; exact/andP.
+Qed.
+
+Lemma is_trace_rcons s st : 
+  is_trace (rcons s st) = [&& is_step st, is_trace s & joint s [:: st]].
+Proof. 
+  rewrite /is_trace all_rcons -andbA -andbA.
+  apply/andb_id2l=> _; apply/andb_id2l=> _.
+  rewrite (sorted_rcons s (rev_lnk st)). 
+  by rewrite /joint.
+Qed.
+                         
+Lemma states_cons st s : joint [:: st] s ->
+  states (st :: s) = src st :: dst st :: behead (states s).
+Proof. admit. Admitted.
+    
+Lemma behead_states s :
+  behead (states s) = map dst s.
+Proof. by rewrite /states; case: s. Qed. 
+
+Lemma states_rcons_src s st : 
+  states (rcons s st) = (map src s) ++ [:: src st; dst st].
+Proof. admit. Admitted.
+
+Lemma states_rcons s st : ~~ nilp s -> is_trace s -> joint s [:: st] ->
+  states (rcons s st) = rcons (states s) (dst st).
+Proof. 
+  move=> /(elimN nilP).
+  case: (lastP s)=> //=.
+  move=> {}s st' _.
+  rewrite is_trace_rcons=> /andP[Htr Hj]. 
+  rewrite joint_rcons /joint /= => Hlnk.
+  rewrite !states_rcons_src map_rcons.
+  rewrite -cats1 -cats1 -catA -catA /=.
+  by move: Hlnk; rewrite /lnk=> /eqP ->.
+Qed.  
+
+Lemma states_cat s1 s2 : ~~ nilp s1 -> is_trace s1 -> joint s1 s2 -> 
+  states (s1 ++ s2) = states s1 ++ behead (states s2).
+Proof. 
+  rewrite behead_states; move=> /(elimN nilP).
+  move: s2; elim/last_ind: s1=> [|{}s1 st IH] s2 _ //=.
+  case: (nilp s1)/nilP=> [->|Hnil] //=.
+  rewrite is_trace_rcons=> /andP[Hs /andP[Htr Hj]].
+  rewrite joint_rcons cat_rcons IH //. 
+  rewrite states_rcons ?cat_rcons //=; exact/nilP.
+Qed.
+
+End Theory.
+
+End Trace.
 
 
 Module Export Simulation.
@@ -237,8 +400,20 @@ Proof. case: R=> ? [[H]] /=; exact/H. Qed.
 (* Proof. admit. Admitted. *)
 
 Lemma sim_traces R s t : 
-  R s t -> lts_lang s ≦ lts_lang t.
-Proof. admit. Admitted.
+  R s t -> ltslang s ≦ ltslang t.
+Proof. 
+  move=> HR w [[tr Htr]] [->]; clear w. 
+  rewrite /ltslang /traces_at /=.
+  rewrite /labels /= => /eqP.
+  move: Htr; elim/last_ind: tr=> [|{}tr st IH] /=.
+  - by exists [trace] => /=.
+  rewrite is_trace_rcons=> /andP[Hs /andP[Htr Hj]].
+  case: (nilp tr)/nilP=> [->|Hnil] /=.
+  - admit.
+  rewrite states_rcons //; last exact/nilP.
+  rewrite headI /=.  
+  admit. 
+Admitted.
 
 End Theory.
 
