theories/common/utils.v
@@ -461,7 +461,7 @@ End SubTypeUtils.
 Section SeqUtils.
 
 Context {T : Type}. 
-Implicit Types (p : pred T) (s : seq T) (n : nat).
+Implicit Types (p : pred T) (r : rel T) (s : seq T) (n : nat).
 
 Lemma hasNcount p s : 
    ~~ has p s = (count p s == 0).
@@ -512,6 +512,14 @@ Qed.
 Lemma find_take p s n : 
   has p (take n s) -> find p (take n s) = find p s. 
 Proof. by rewrite -[in find p s](@cat_take_drop n _ s) find_cat=> ->. Qed.
+
+Lemma sorted_rcons x r s y : 
+  r x y -> sorted r (rcons s y) = sorted r s && r (last x s) y.
+Proof. 
+  move=> Hxy; case s=> [|z {}s] /=. 
+  - by rewrite Hxy. 
+  exact/rcons_path.
+Qed.
 
 Lemma sorted_subn (s : seq nat) n : 
   sorted ltn s -> all (fun m => n <= m) s -> sorted ltn (map (subn^~ n) s).  
